zero = x(X).x(s).x(z).z<->x
one = x(X).x(s).x(z).?s[f].f[a].(a<->z|f<->x)

count = x[? Top] . x[s] . (!s(f) . f(a) . incr | x[z] . (nought | x <-> y))

-- countZero = \x . (zero | count)
-- countOne = \x . (one | count)

\x.
  x(X).x(s).x(z).?s[f].f[a].(a<->z|f<->x)
  x[? Top] . x[s] . (!s(f) . f(a) . incr{z,y} | x[z] . (nought{z} | x <-> y))

=> IO

\x.
  x[s] . (!s(f) . f(a) . incr | x[z] . (nought | x <-> y))    {x}
  x(s).x(z).?s[f].f[a].(a<->z|f<->x)                          {x}

=> s

\s.
  !s(f) . f(a) . incr                   {s}
  \x.
    x[z] . (nought | x <-> y)           {s x}
    x(z).?s[f].f[a].(a<->z|f<->x)       {s x}

=> z

\s.
  \z
    nought                              {s z}
    \x.
      x <-> y                           {s z x}
      ?s[f].f[a].(a<->z|f<->x)          {s z x}
  !s(f) . f(a) . incr                   {s}

=> assoc

\z
  nought                                {z}
  \s
    \x.
      x <-> y                           {z s x}
      ?s[f].f[a].(a<->z|f<->x)          {z s x}
    !s(f) . f(a) . incr                 {z s}

=> assoc

\z
  nought                                {z}
  \x
    x <-> y                             {z x}
    \s.
      !s(f) . f(a) . incr               {z x s}
      ?s[f].f[a].(a<->z|f<->x)          {z x s}

=> !?


\z
  nought                                {z}
  \x
    x <-> y                             {z x}
    \f.
      f(a) . incr                       {z x f}
      f[a] . (a<->z|f<->x)              {z x f}

=> a

\z
  nought                                {z}
  \x
    x <-> y                             {z x}
    \a
      a<->z                             {z x a}
      \f
        f<->x                           {z x a f}
        incr                            {z x a f}

=>

\z
  nought                                {z}
  incr {y}

======================================================



\x.
  x[s] . (!s(f) . f(a) . incr{af} | x[z] . (nought{z} | x <-> y))    {x y}
  x(s).x(z).?s[f].f[a].(a<->z|f<->x)                                 {x}

=> x > s

\s
  !s(f) . f(a) . incr{af}                 {s}
  \x
    x[z] . (nought{z} | x <-> y)          {x y}
    x(z). ?s[f] . f[a] . (a<->z|f<->x)    {x s}

=> x > z

\s
  !s(f) . f(a) . incr{af}             {s}
  \z
    nought{z}                         {z}
    \x
      x <-> y                         {x y}
      ?s[f] . f[a] . (a<->z|f<->x)    {x s z}

=> x <-> y

\s
  !s(f) . f(a) . incr{af}             {s}
  \z
    nought{z}                         {z}
    ?s[f] . f[a] . (a<->z|f<->y)      {y s z}

=> assoc


\s
  !s(f) . f(a) . incr{af}             {s}
  \z
    nought{z}                         {z}
    ?s[f] . f[a] . (a<->z|f<->y)      {y s z}

=> assoc

\z
  nought{z}                         {z}
  \s
    !s(f) . f(a) . incr{af}           {s}
    ?s[f] . f[a] . (a<->z|f<->y)      {y s z}

=> !?

\z
  nought{z}                 {z}
  \f
    f(a) . incr{af}           {f}
    f[a] . (a<->z|f<->y)      {y f z}

=> f > a

\z
  nought{z}                 {z}
  \a
    a<->z   {a z}
    \f
      incr{af}           {f}
      f<->y               {y f z}

=> f <-> y

\z
  nought{z}                 {z}
  incr{z y}                 {z y}
